\documentclass{article}
\usepackage{amsmath}
\usepackage{amsfonts}
\usepackage{latexsym}
\usepackage{graphicx}
\newcommand{\comment}[1]{}
\newcommand{\field}[1]{\mathbb{#1}} % requires amsfonts
\newcommand{\pd}[2]{\frac{\partial#1}{\partial#2}}
\begin{document}
\title{HW6, Classical Electromagnetism, Fall 2016}
\author{Deheng Song}
\maketitle

\section*{Jackson 3.16(b)}
\[ \nabla^2\frac{1}{|\vec x-\vec x'|}=-4\pi\delta(\vec x-\vec x')=-\frac{4\pi}{\rho}\delta(\rho-\rho')\delta(\phi-\phi')\delta(z-z') \]
Expand,
\begin{align*}
  \frac{1}{\rho}\delta(\rho-\rho')=\int_0^\infty kJ_m(k\rho)J_m(k\rho')dk\\
  \delta(\phi-\phi')=\frac{1}{2\pi}\sum_{m=-\infty}^{\infty} e^{im(\phi-\phi')}
\end{align*}
Let,
\begin{align*}
  \frac{1}{|\vec x-\vec x'|}=-2\sum_{m=-\infty}^\infty\int_0^{\infty}dk e^{im(\phi-\phi')}kJ_m(k\rho)J_m(k\rho')g(k,z,z')
\end{align*}
The Laplace equation then becomes,
\begin{align*}
  &-2\sum_{m=-\infty}^\infty\int_0^\infty  dk[\frac{1}{\rho}\pd{}{\rho}\rho\pd{}{\rho}+\frac{1}{\rho^2}\pd{^2}{\phi^2}+\pd{^2}{z^2}]e^{im(\phi-\phi')}kJ_m(k\rho)J_m(k\rho')g(k,z,z')\\
  =&-2\sum_{m=-\infty}^\infty\int_0^\infty  dk[(\frac{1}{\rho}\pd{}{\rho}\rho\pd{J_m(k\rho)}{\rho}-\frac{m^2}{\rho^2}J_m(k\rho))g(k,z,z')\\
  &+J_m(k\rho)\pd{^2g(k,z,z')}{z^2}]e^{im(\phi-\phi')}kJ_m(k\rho')\\
  =&-\frac{4\pi}{\rho}\delta(\rho-\rho')\delta(\phi-\phi')\delta(z-z')
\end{align*}
Since $J_m(k\rho)$ satisfies the Bessel equation, we find
\[ \frac{1}{\rho}\pd{}{\rho}\rho\pd{J_m(k\rho)}{\rho}-\frac{m^2}{\rho^2}J_m(k\rho)=-k^2J_m(k\rho) \]
Insert to the equation above,
\begin{align*}
  &-2\sum_{m=-\infty}^\infty\int_0^\infty  dk[\pd{^2g(k,z,z')}{z^2}-k^2g(k,z,z')] e^{im(\phi-\phi')}kJ_m(k\rho)J_m(k\rho')\\
  =&-\frac{4\pi}{\rho}\delta(\rho-\rho')\delta(\phi-\phi')\delta(z-z')
\end{align*}
It demands,
\begin{align*}
  \pd{^2g(k,z,z')}{z^2}-k^2g(k,z,z')=-4\pi\delta(z-z')
\end{align*}
When $z\neq z'$, the general solution is given by,
\begin{align*}
  g(z,z')= Ae^{k(z-z')}+Be^{-k(z-z')}
\end{align*}
When $z>z'$, we want $g(z,z')$ vanishes at $z\rightarrow\infty$, and when $z<z'$ we want $g(z,z')$ vanishes at $z\rightarrow -\infty$, hence we have
\[ A=0\ when\ z>z',\qquad B=0\ when\ z<z' \]
At $z=z'$, $e^{-k(z-z')}=e^{k(z-z')}=1$, we have
\[ A=B \]
The general solution can be writen as
\[ g(z,z')=Ae^{-k(z_>-z_<)} \]
Now consider the discontinuity of the first derivative at $z=z'$,
\[ \pd{g}{z}|_{z=z'+}-\pd{g}{z}|_{z=z'-}=-4\pi \]
\[ A=\frac{2\pi}{k} \]
Finally we have,
\[ \boxed{\frac{1}{|\vec x-\vec x'|}=\sum_{m=-\infty}^{\infty}\int_0^{\infty}dk e^{im(\phi-\phi')}J_m(k\rho)J_m(k\rho')e^{-k(z_>-z_<)}} \]\par
\pagebreak

\section*{Jackson 3.16(c)}

When $\rho'=0$ and $z'=0$,
\[ \frac{1}{|\vec x-\vec x'|}=\frac{1}{\sqrt{\rho^2+z^2}} \]
which has azimuthal symmetry. $m=0$.
We have
\[ J_0(0)=1 \]
\[e^{-k(z_>-z_<)}=e^{-k|z|} \]
\begin{align*}
  \frac{1}{\sqrt{\rho^2+z^2}}=\int_0^{\infty} e^{-k|z|}J_0(k\rho)dk
\end{align*}\par
Let $z=z'$ and $\phi'=0$, replace $R^2=\rho^2+\rho'^2-\rho\rho'\cos\phi$, and we find
\begin{align*}
  \frac{1}{|\vec x-\vec x'|}=\frac{1}{\sqrt{\rho^2+\rho'^2-2\rho\rho'\cos\phi}}=\int_0^\infty J_0(k\sqrt{\rho^2+\rho'^2-2\rho\rho'\cos\phi}) dk\\
  =\int_0^\infty\sum_{m=-\infty}^{\infty}e^{im\phi}J_m(k\rho)J_m(k\rho')dk
\end{align*}
Thus,
\[ J_0(k\sqrt{\rho^2+\rho'^2-2\rho\rho'\cos\phi})=\sum_{m=-\infty}^{\infty}J_m(k\rho)J_m(k\rho')dk\]
The generating function of $J_n(x)$ is
\[ e^{\frac x2(z-z^{-1})}=\sum_{n=-\infty}^{\infty}J_n(x)z^n \]
In this case, $z=ie^{i\phi}$ and $x=k\rho$, we get
\begin{align*}
  e^{\frac{k\rho}{2}(ie^{i\phi}-\frac{1}{ie^{i\phi}})}=e^{ik\rho\cos\phi}=\sum_{m=-\infty}^{\infty}i^m e^{im\phi} J_m(k\rho)
\end{align*}
\pagebreak

\section*{Jackson 3.16(d)}

From the last result,
 \[ e^{ix\cos\phi}=\sum_{m=-\infty}^{\infty}i^m e^{im\phi} J_m(x) \]
 Multiply both sides by $e^{-im\phi'}$ and integral from $0$ to $2\pi$, we get
\begin{align*}
   \int_0^{2\pi} e^{ix\cos\phi-im\phi'} d\phi &= \sum_{m=-\infty}^{\infty}\int_0^{2\pi} i^m e^{im(\phi-\phi')}J_m(x) d\phi\\
                                              &=2\pi\int_0^{2\pi}i^m J_m(x)\delta(\phi-\phi')d\phi
\end{align*}
The right side is nontrival only when $\phi=\phi'$, in this case,
\[ J_m(x)=\frac{1}{2\pi i^m}\int_0^{2\pi}e^{ix\cos\phi-im\phi}d\phi \]
\pagebreak

\section*{Jackson 3.17(a)}

Since the green function vanishes at $z=0$ and $z=L$, we can write,
\[ G(\vec x,\vec x')=\sum_{m,n}g(\rho,\rho')e^{im(\phi-\phi')}\sin(\frac{n\pi z}{L})\sin(\frac{n\pi z'}{L}) \]
The green fucntion satisfies,
\[[\frac{1}{\rho}\pd{}{\rho}\rho\pd{}{\rho}+\frac{1}{\rho^2}\pd{^2}{\phi^2}+\pd{^2}{z^2}]G(\rho,\rho';\phi,\phi';z,z')=-\frac{4\pi}{\rho}\delta(\rho-\rho')\delta(\phi-\phi')\delta(z-z') \]
Since,
\[\delta(\phi-\phi')=\frac{1}{2\pi}\sum_{m=-\infty}^{\infty}e^{im(\phi-\phi')} \]
\[\delta(z-z')=\frac{2}{L}\sum_{n=1}^\infty \sin(n\pi z/L)\sin(n\pi z'\L) \]
We want
\[ [\frac{1}{\rho}\pd{}{\rho}\rho\pd{}{\rho}-\frac{m^2}{\rho^2}-(\frac{n\pi}{L})^2]g(\rho,\rho')=-\frac{4}{L\rho}\delta(\rho-\rho') \]
which is a modified Bessel equation. The solution for $g(\rho,\rho')$ satisfies,
\[ g_<=g_>\quad when\ \rho=\rho'\]
\[ \frac{dg}{d\rho}|_{\rho=\rho+}-\frac{dg}{d\rho}|_{\rho=\rho-}=-\frac{4}{n\pi\rho} \]
From the Wronskian formula,
\[ I_v(\rho)K_v'(\rho)-I_v'(\rho)K_v(\rho)=\frac{-L}{n\pi\rho} \]
which gives the solution
\[ g(\rho,\rho')=\frac{4}{L}I_m(\frac{n\pi\rho_<}{L})K_m(\frac{n\pi\rho'}{L})\]
Finally,
\[ \boxed{G(\vec x,\vec x')=\frac{4}{L}\sum_{n=1}^{\infty}\sum_{m=-\infty}^\infty e^{im(\phi-\phi')}\sin(\frac{n\pi z}{L})\sin(\frac{n\pi z'}{L})I_m(\frac{n\pi\rho}{L})K_m(\frac{n\pi\rho'}{L})}\]
\pagebreak

\section*{Jackson 3.7(b)}

Expand the Green fucntion in terms of $\rho$ and $\phi$,
\[ G(\vec x,\vec x')=\sum_{m=-\infty}^\infty\int_0^{\infty}dk kg(k,z,z')e^{im(\phi-\phi')}J_m(k\rho)J_m(k\rho') \]
As showed in 3.6(b), we have
\[ \pd{^2g(z,z')}{z^2}-k^2g(z,z')=-2\delta(z-z') \]
The boudary conditions require $g(z,z')=0$ at $z=0$ and $z=L$. When $z<z'$,
\[ g(z,z')=A\sinh(kz) \]
When $z>z'$,
\[ g(z,z')=B\sin[k(L-z)] \]
And
\[ A\sin(kz')=B\sin[k(L-z')] \]
\[ -B\cosh[k(L-z')]-A\cosh(kz')=-\frac{2}{k}\]
Then we can solve,
\[ A=\frac{2\sinh[k(L-z')]}{2\sinh(kL)}\qquad B=\frac{2\sinh(kz')}{k\sinh(kL)}\]
and write $g(z,z')$ as
\[ g(z,z')=\frac{2\sinh(kz_<)\sin[k(L-z_>)]}{k\sinh(kL)} \]
The Green fucntion,
\[ \boxed{G(\vec x,\vec x')=2\sum_{m=-\infty}^\infty\int_0^{\infty}dk e^{im(\phi-\phi')}J_m(k\rho)J_m(k\rho')\frac{\sinh(kz_<)\sin[k(L-z_>)]}{\sinh(kL)}}\]
\pagebreak

\section*{Jackson 4.2}

The potential caused by a dipole is
\begin{align*}
  \Phi(\vec x)&=\frac{\vec p\cdot\vec x}{4\pi\varepsilon_0|\vec x-\vec x'|^3}\\
              &=-\frac{\vec p}{4\pi\varepsilon_0}\nabla\frac{1}{|\vec x-\vec x'|}\\
              &=\frac{1}{4\pi\varepsilon_0}\int\frac{\rho(\vec x')}{|\vec x-\vec x'|}d^3x'
\end{align*}
We want
\[ \int\frac{\rho(\vec x')}{|\vec x-\vec x'|}d^3x'=-\vec p\cdot\nabla\frac{1}{|\vec x-\vec x'|} \]
\begin{align*}
  [-\vec p\cdot\nabla\frac{1}{|\vec x-\vec x'|}]|_{x=x_0}&=-\int\delta(\vec x-\vec x_0)\vec p\cdot\nabla\frac{1}{|\vec x-\vec x'|}d^3x=-\int\frac{\rho(\vec x)}{|\vec x-\vec x_0|}d^3x
\end{align*}
Integral by parts we find,
\begin{align*}
  \int\frac{1}{|\vec x-\vec x_0|}\vec p\cdot\nabla(\delta(\vec x-\vec x_0))d^3x=-\int\frac{\rho(\vec x)}{|\vec x-\vec x_0|}d^3x
\end{align*}
Hence we have
\[ \boxed{\rho(x)=-\vec p\cdot\nabla\delta(\vec x-\vec x_0)}\]
Similarly, the electtrostatic energy of a dipole is
\[ W=-\vec p\cdot E(0)=\vec p\cdot\nabla\Phi(0)=\int\rho(\vec x)\Phi(\vec x)d^3x \]
\begin{align*}
  \int\delta(\vec x-\vec x_0)\vec p\cdot\nabla\Phi(\vec x)d^3&=-\int\Phi(\vec x)\vec p\cdot\nabla(\delta(\vec x-\vec x_0))d^3x\\
                                                             &=\int\rho(\vec x)\Phi(\vec x)d^3x
\end{align*}
Hence,
\[ \boxed{\rho(x)=-\vec p\cdot\nabla\delta(\vec x-\vec x_0)}\]
\pagebreak

\section*{Jackson 4.7(a)}

\begin{align*}
  \rho(\vec r)&=\frac{1}{64\pi}r^2e^{-r}\sin^2\theta\\
              &=\frac{1}{96\pi}r^2e^{-r}[P_0(\cos\theta)-P_2(\cos\theta)]
\end{align*}
The charge distribution has azimuthal symmetry, all $m\neq0$ terms vanishes.
\[ Y_{l0}=\sqrt{\frac{2l+1}{4\pi}}P_l(\cos\theta) \]
The multipole expansions
\begin{align*}
  \Phi(\vec r)&=\frac{1}{96\pi}\frac{1}{4\pi\varepsilon_0}\sum_{l}[\int_0^{2\pi}d\phi \int_0^\infty\int_{-1}^{1}P_l(\cos\theta')r'^{l+4}e^{-r}[P_0(\cos\theta)-P_2(\cos\theta)]drd\cos\theta]\frac{P_l(\cos\theta)}{r^{l+1}}\\
              &=\frac{1}{48}\frac{1}{4\pi\varepsilon_0}[\Gamma(l+5)(2\delta_{l0}-\frac 25 \delta_{l2})]\frac{P_l(\cos\theta)}{r^{l+1}}\\
              &=\frac{1}{4\pi}[\frac{P_0(\cos\theta)}{r}-6\frac{P_2(\cos\theta)}{r^3}]
\end{align*}

\section*{Jackson 4.7(b)}
Under azimuthal symmetry, the Green function can be expanded in
\[ G(\vec x, \vec x')=\sum_{l=0}^\infty\frac{r_<^l}{r_>^{l+1}}P_l(\cos\theta)P_l(\cos\theta') \]
The potential at any point,
\begin{align*}
  \Phi(\vec x)&=\frac{1}{48}\frac{1}{4\pi\varepsilon_0}\int_0^\infty r'^4e^{-r'}\frac{r_<^l}{r_>^{l+1}}dr'\int_{-1}^{1}[P_0(\cos\theta')-P_2(\cos\theta')]P_l(\cos\theta')P_l(\cos\theta)d\cos\theta'\\
              &=\frac{1}{48}\frac{1}{4\pi\varepsilon_0}[\frac{1}{r^{l+1}}\int_0^r r'^{l+4}e^{-r'}dr'+r^l\int_0^\infty \frac{r'^3}{r'^l}e^{-r'}dr'][2\delta_{l0}P_0(\cos\theta)-\frac{2}{5}\delta_{l2}P_2(\cos\theta)]\\
              &=\frac{1}{24}\frac{1}{4\pi\varepsilon_0}[\frac{P_0(\cos\theta)}{r}(24-e^{-r}(24+18r+6r^2+r^3))\\
              &-\frac{P_2(\cos\theta)}{r^3}(144-e^{-r}(144+144r+72r^2+24r^3+6r^4+r^5))]
\end{align*}
When $r\rightarrow\infty$, $e^{-r}\rightarrow 0$, the potential above reduces to the form in (a). When $r\rightarrow 0$, expand
\[e^{-r}=1-r+\frac{1}{2}r^3-\frac{1}{6}r^3+\frac{1}{24}r^4-\frac{1}{120}r^5...\]
Insert to the potential and calculate to the $r^2$ terms,
\begin{align*}
  \Phi(\vec x)&=\frac{1}{24}\frac{1}{4\pi\varepsilon_0}[\frac{1}{r}(6r+\frac{r^5}{20}+...)-\frac{P_2(\cos\theta)}{r^3}(\frac{r^5}{5}+\frac{r^6}{5}...)]\\
              &=\frac{1}{4\pi\varepsilon_0}[\frac{1}{4}-\frac{r^2}{120}P_2(\cos\theta)]
\end{align*}
% \bibliographystyle{abbrv}
% \bibliography{refs}
\end{document}